examples/tactics/Syntax.fst
@@ -9,7 +9,7 @@ let test1 = assert_by_tactic (pack (Tv_Const (C_Int ((10 + 8) + (3 + 9))));;
 let test2 = assert_by_tactic (x <-- quote test1;
                               v <-- inspect x;
                               match v with
-                              | Tv_FVar fv -> print ("FV: " ^ inspectfv fv)
+                              | Tv_FVar fv -> print ("FV: " ^ flatten_gname (inspect_fv fv))
                               | _ -> fail "wat") True
 
 
@@ -17,7 +17,7 @@ let blah : term -> tactic term = fix1 (fun ff t ->
     tv <-- inspect t;
     tv <-- (match tv with
            | Tv_Var b -> return (Tv_Var b)
-           | Tv_FVar f -> print ("FVar = " ^ inspectfv f);;
+           | Tv_FVar f -> print ("FVar = " ^ flatten_gname (inspect_fv f));;
                           return (Tv_FVar f)
            | Tv_App l r -> l <-- ff l;
                            r <-- ff r;
@@ -38,3 +38,12 @@ let _ = assert_by_tactic (t <-- quote (1+1);
                           s <-- term_to_string t; print ("t = " ^ s);;
                           return ()
                           ) True
+
+let _ = assert_by_tactic (t <-- quote blah;
+                          tv <-- inspect t;
+                          (match tv with
+                          | Tv_FVar fv ->
+                              print (flatten_gname (inspect_fv fv));;
+                              return ()
+                          | _ ->
+                              fail "wat")) True
